CookLevin/Complexity.lean
@@ -3,6 +3,8 @@ import Complexity.Complexity.TMDecider
 import Complexity.Complexity.TMEncoding
 import Complexity.Complexity.TMPrimitives
 import Complexity.Complexity.Deciders.SAT_TM
+import Complexity.Complexity.Deciders.EvalCnfTM
+import Complexity.Complexity.Deciders.CliqueRelTM
 import Complexity.NP.SAT.CookLevin
 
 set_option autoImplicit false
